Add context weakening and prove typing for locks

F_mu_ref_par/examples/lock.v
@@ -1,5 +1,5 @@
 From iris.proofmode Require Import invariants ghost_ownership tactics.
-From F_mu_ref_par Require Import lang rules rules_binary.
+From F_mu_ref_par Require Import lang rules rules_binary typing.
 Import uPred.
 
 Definition newlock : expr := Alloc (♭ false).
@@ -17,9 +17,99 @@ Definition with_lock (e : expr) (l : expr) : expr :=
     l
 .
 
+Lemma newlock_closed f : newlock.[f] = newlock.
+Proof. by asimpl. Qed.
+
+Lemma acquire_closed f : acquire.[f] = acquire.
+Proof. by asimpl. Qed.
+
+Lemma release_closed f : release.[f] = release.
+Proof. by asimpl. Qed.
+
+Lemma with_lock_closed e l:
+  (∀ f : var → expr, e.[f] = e) →
+  (∀ f : var → expr, l.[f] = l) →
+  ∀ f, (with_lock e l).[f] = with_lock e l.
+Proof. asimpl => H1 H2 f. by rewrite H1 H2. Qed.
+
+Definition LockType := Tref TBool.
+
+Lemma newlock_type Γ : typed Γ newlock LockType.
+Proof. repeat constructor. Qed.
+
+Lemma acquire_type Γ : typed Γ acquire (TArrow LockType TUnit).
+Proof. do 3 econstructor; eauto using EqTBool; repeat constructor. Qed.
+
+Lemma release_type Γ : typed Γ release (TArrow LockType TUnit).
+Proof. repeat econstructor. Qed.
+
+Lemma with_lock_type e l Γ τ :
+  (∀ f : var → expr, e.[f] = e) →
+  typed Γ e (TArrow TUnit τ) →
+  typed Γ l LockType →
+  typed Γ (with_lock e l) TUnit.
+Proof.
+  intros H1 H2 H3. econstructor; eauto.
+  repeat (econstructor; eauto using release_type, acquire_type).
+  eapply (closed_context_weakening [_; _; _; _]); eauto.
+Qed.
+
 Section proof.
   Context {Σ : gFunctors} {iS : cfgSG Σ}.
-  Context (S : namespace).
+
+  Lemma steps_newlock N E ρ j K :
+    nclose N ⊆ E →
+    (((Spec_ctx N ρ ★ j ⤇ (fill K (newlock)))%I)
+      ⊢ |={E}=>(∃ l, j ⤇ (fill K (Loc l)) ★ l ↦ₛ (♭v false))%I).
+  Proof.
+    intros HNE.
+    iIntros "[#Hspec Hj]".
+    iPvs (step_alloc _ _ _ j K _ _ _ _ with "[Hj]") as "Hj"; eauto.
+    iFrame "Hspec Hj"; trivial.
+    Unshelve. all: trivial.
+  Qed.
+
+  Global Opaque newlock.
+
+  Lemma steps_acquire N E ρ j K l :
+    nclose N ⊆ E →
+    (((Spec_ctx N ρ ★ l ↦ₛ (♭v false) ★ j ⤇ (fill K (App acquire (Loc l))))%I)
+      ⊢ |={E}=>(j ⤇ (fill K Unit) ★ l ↦ₛ (♭v true))%I).
+  Proof.
+    intros HNE.
+    iIntros "[#Hspec [Hl Hj]]". unfold acquire.
+    iPvs (step_lam _ _ _ j K _ _ _ _ with "[Hj]") as "Hj"; eauto.
+    iFrame "Hspec Hj"; trivial. simpl.
+    iPvs (step_cas_suc _ _ _ j (K ++ [IfCtx _ _])
+                       _ _ _ _ _ _ _ _ _ with "[Hj Hl]") as "[Hj Hl]"; trivial.
+    rewrite ?fill_app. simpl.
+    iFrame "Hspec Hj Hl"; trivial.
+    iNext; trivial.
+    rewrite ?fill_app. simpl.
+    iPvs (step_if_true _ _ _ j K _ _ _ with "[Hj]") as "Hj"; trivial.
+    iFrame "Hspec Hj"; trivial.
+    iPvsIntro. iFrame "Hj Hl"; trivial.
+    Unshelve. all:trivial.
+  Qed.
+
+  Global Opaque acquire.
+
+  Lemma steps_release N E ρ j K l b:
+    nclose N ⊆ E →
+    (((Spec_ctx N ρ ★ l ↦ₛ (♭v b) ★ j ⤇ (fill K (App release (Loc l))))%I)
+      ⊢ |={E}=>(j ⤇ (fill K Unit) ★ l ↦ₛ (♭v false))%I).
+  Proof.
+    intros HNE.
+    iIntros "[#Hspec [Hl Hj]]". unfold release.
+    iPvs (step_lam _ _ _ j K _ _ _ _ with "[Hj]") as "Hj"; eauto.
+    iFrame "Hspec Hj"; trivial. simpl.
+    iPvs (step_store _ _ _ j K _ _ _ _ _ with "[Hj Hl]") as "[Hj Hl]"; eauto.
+    iFrame "Hspec Hj"; trivial.
+    iPvsIntro. iFrame "Hj Hl"; trivial.
+    Unshelve. all: trivial.
+  Qed.
+
+  Global Opaque release.
 
   Lemma steps_with_lock N E ρ j K e l P Q :
     nclose N ⊆ E →
@@ -28,55 +118,37 @@ Section proof.
     (∃ v, ∀ K', ((Spec_ctx N ρ ★ P ★ j ⤇ (fill K' (App e Unit)))%I)
             ⊢ |={E}=>(j ⤇ (fill K' (of_val v)) ★ Q)%I)
     →
-    (((Spec_ctx N ρ ★ P ★ l ↦ₛ (♭v false) ★ j ⤇ (fill K (with_lock e (Loc l))))%I)
+    (((Spec_ctx N ρ ★ P ★ l ↦ₛ (♭v false)
+                ★ j ⤇ (fill K (with_lock e (Loc l))))%I)
       ⊢ |={E}=>(j ⤇ (fill K (Unit)) ★ Q ★ l ↦ₛ (♭v false))%I).
   Proof.
     intros HNE H1 [v H2].
     iIntros "[#Hspec [HP [Hl Hj]]]".
     iPvs (step_lam _ _ _ j K _ _ _ _ with "[Hj]") as "Hj"; eauto.
+    iFrame "Hspec Hj"; trivial. simpl.
+    rewrite acquire_closed release_closed H1. asimpl.
+    iPvs (steps_acquire _ _ _ j (K ++ [AppRCtx (LamV _)])
+                   _ _ with "[Hj Hl]") as "[Hj Hl]"; eauto.
+    rewrite fill_app; simpl.
     iFrame "Hspec Hj"; trivial.
-    asimpl.
-    Unshelve. 3: simpl; auto.
-    iPvs (step_lam _ _ _ j (K ++ [AppRCtx (LamV _)])
-                   _ _ _ _ with "[Hj]") as "Hj"; eauto.
-    rewrite fill_app. simpl.
-    iFrame "Hspec Hj"; trivial.
-    Unshelve. 3: simpl; trivial.
-    asimpl.
-    iPvs (step_cas_suc _ _ _ j (K ++ [AppRCtx (LamV _); IfCtx _ _])
-                       _ _ _ _ _ _ _ _ _ with "[Hj Hl]") as "[Hj Hl]"; trivial.
-    rewrite ?fill_app. simpl.
-    iFrame "Hspec Hj Hl"; trivial.
-    Unshelve. 7: simpl; trivial. 5: simpl; trivial. 4: trivial.
-    iNext; trivial.
-    rewrite fill_app. simpl.
-    iPvs (step_if_true _ _ _ j (K ++ [AppRCtx (LamV _)])
-                       _ _ _ with "[Hj]") as "Hj"; trivial.
-    rewrite ?fill_app. simpl.
-    iFrame "Hspec Hj"; trivial.
-    rewrite fill_app. simpl.
-    Unshelve. all: trivial.
+    rewrite fill_app; simpl.
     iPvs (step_lam _ _ _ j K _ _ _ _ with "[Hj]") as "Hj"; eauto.
-    iFrame "Hspec Hj"; trivial.
-    asimpl.
-    Unshelve. 3: simpl; auto.
-    rewrite H1.
+    iFrame "Hspec Hj"; trivial. asimpl.
+    rewrite release_closed H1.
     iPvs (H2 (K ++ [AppRCtx (LamV _)]) with "[Hj HP]") as "[Hj HQ]"; eauto.
     rewrite ?fill_app. simpl.
     iFrame "Hspec Hj"; trivial.
     rewrite ?fill_app. simpl.
     iPvs (step_lam _ _ _ j K _ _ _ _ with "[Hj]") as "Hj"; eauto.
-    iFrame "Hspec Hj"; trivial.
-    asimpl.
-    Unshelve. 3: auto using to_of_val.
-    iPvs (step_lam _ _ _ j K _ _ _ _ with "[Hj]") as "Hj"; eauto.
-    iFrame "Hspec Hj"; trivial.
-    asimpl.
-    Unshelve. 3: simpl; auto.
-    iPvs (step_store _ _ _ j K _ _ _ _ _ with "[Hj Hl]") as "[Hj Hl]"; eauto.
-    iFrame "Hspec Hj"; trivial.
-    Unshelve. 3: auto.
-    iPvsIntro. iFrame "HQ Hj Hl"; trivial.
+    iFrame "Hspec Hj"; trivial. simpl.
+    rewrite release_closed.
+    iPvs (steps_release _ _ _ j K _ _ with "[Hj Hl]") as "[Hj Hl]"; eauto.
+    iFrame "Hspec Hl Hj"; trivial.
+    iPvsIntro. iFrame "Hj HQ Hl"; trivial.
+    Unshelve.
+    all: try match goal with |- to_val _ = _ => auto using to_of_val end.
+    trivial.
   Qed.
 
+  Global Opaque with_lock.
 End proof.
